remove (V)Param(')

Qdt/Theory/Substitution/Basic.lean
@@ -29,16 +29,16 @@ mutual
 
 def Ty.subst {m n : Nat} (σ : Subst m n) : Ty m → Ty n
   | .u i => .u i
-  | .pi ⟨x, a⟩ b => .pi ⟨x, a.subst σ⟩ (b.subst σ.up)
+  | .pi x a b => .pi x (a.subst σ) (b.subst σ.up)
   | .el t => .el (t.subst σ)
 
 def Tm.subst {m n : Nat} (σ : Subst m n) : Tm m → Tm n
   | .u' i => .u' i
   | .var i => σ i
   | .const name us => .const name us
-  | .lam ⟨x, a⟩ body => .lam ⟨x, a.subst σ⟩ (body.subst σ.up)
+  | .lam x a body => .lam x (a.subst σ) (body.subst σ.up)
   | .app f a => .app (f.subst σ) (a.subst σ)
-  | .pi' ⟨x, a⟩ b => .pi' ⟨x, a.subst σ⟩ (b.subst σ.up)
+  | .pi' x a b => .pi' x (a.subst σ) (b.subst σ.up)
   | .proj i t => .proj i (t.subst σ)
   | .letE x ty t body => .letE x (ty.subst σ) (t.subst σ) (body.subst σ.up)
 
@@ -61,7 +61,7 @@ mutual
 theorem Ty.ren_eq_subst_var {m n} (ξ : Ren m n) :
     ∀ A : Ty m, A.ren ξ = A.subst ξ.toSubst
   | .u .. => rfl
-  | .pi ⟨_, _⟩ _ => by
+  | .pi _ _ _ => by
     simp only [Ty.ren, Ty.subst, Ty.ren_eq_subst_var, Subst.subst_comp_up]
   | .el t => by simp only [Ty.ren, Ty.subst, Tm.ren_eq_subst_var ξ t]
 
@@ -70,10 +70,10 @@ theorem Tm.ren_eq_subst_var {m n} (ξ : Ren m n) :
   | .u' .. => rfl
   | .var _ => rfl
   | .const .. => rfl
-  | .lam ⟨_, _⟩ _ => by
+  | .lam _ _ _ => by
       simp only [Tm.ren, Tm.subst, Ty.ren_eq_subst_var, Tm.ren_eq_subst_var, Subst.subst_comp_up]
   | .app .. => by simp only [Tm.ren, Tm.subst, Tm.ren_eq_subst_var]
-  | .pi' ⟨_, _⟩ _ => by
+  | .pi' _ _ _ => by
       simp only [Tm.ren, Tm.subst, Tm.ren_eq_subst_var, Subst.subst_comp_up]
   | .proj .. => by simp only [Tm.ren, Tm.subst, Tm.ren_eq_subst_var]
   | .letE .. => by
@@ -88,7 +88,7 @@ mutual
 @[simp]
 theorem Ty.subst_id {n} : ∀ A : Ty n, A.subst (Subst.id n) = A
   | .u .. => rfl
-  | .pi ⟨_, _⟩ _ => by simp [Ty.subst, Ty.subst_id]
+  | .pi _ _ _ => by simp [Ty.subst, Ty.subst_id]
   | .el .. => by simp only [Ty.subst, Tm.subst_id]
 
 @[simp]
@@ -96,9 +96,9 @@ theorem Tm.subst_id {n} : ∀ t : Tm n, t.subst (Subst.id n) = t
   | .u' .. => rfl
   | .var _ => rfl
   | .const .. => rfl
-  | .lam ⟨_, _⟩ _ => by simp [Tm.subst, Ty.subst_id, Tm.subst_id]
+  | .lam _ _ _ => by simp [Tm.subst, Ty.subst_id, Tm.subst_id]
   | .app .. => by simp [Tm.subst, Tm.subst_id]
-  | .pi' ⟨_, _⟩ _ => by simp [Tm.subst, Tm.subst_id]
+  | .pi' _ _ _ => by simp [Tm.subst, Tm.subst_id]
   | .proj .. => by simp only [Tm.subst, Tm.subst_id]
   | .letE .. => by simp [Tm.subst, Ty.subst_id, Tm.subst_id]
 
@@ -133,7 +133,7 @@ mutual
 theorem Ty.ren_subst {l m n} (ξ : Ren l m) (σ : Subst m n) :
     (A : Ty l) → (A.ren ξ).subst σ = A.subst (σ ∘ ξ)
   | .u .. => rfl
-  | .pi ⟨_, _⟩ _ => by simp only [Ty.ren, Ty.subst, Ty.ren_subst, Subst.comp_ren_up]
+  | .pi _ _ _ => by simp only [Ty.ren, Ty.subst, Ty.ren_subst, Subst.comp_ren_up]
   | .el .. => by simp only [Ty.ren, Ty.subst, Tm.ren_subst]
 
 theorem Tm.ren_subst {l m n} (ξ : Ren l m) (σ : Subst m n) :
@@ -141,9 +141,9 @@ theorem Tm.ren_subst {l m n} (ξ : Ren l m) (σ : Subst m n) :
   | .u' .. => rfl
   | .var _ => rfl
   | .const .. => rfl
-  | .lam ⟨_, _⟩ _ => by simp only [Tm.ren, Tm.subst, Tm.ren_subst, Ty.ren_subst, Subst.comp_ren_up]
+  | .lam _ _ _ => by simp only [Tm.ren, Tm.subst, Tm.ren_subst, Ty.ren_subst, Subst.comp_ren_up]
   | .app .. => by simp only [Tm.ren, Tm.subst, Tm.ren_subst]
-  | .pi' ⟨_, _⟩ _ => by simp only [Tm.ren, Tm.subst, Tm.ren_subst, Subst.comp_ren_up]
+  | .pi' _ _ _ => by simp only [Tm.ren, Tm.subst, Tm.ren_subst, Subst.comp_ren_up]
   | .proj .. => by simp only [Tm.ren, Tm.subst, Tm.ren_subst]
   | .letE .. => by simp only [Tm.ren, Tm.subst, Tm.ren_subst, Ty.ren_subst, Subst.comp_ren_up]
 
@@ -161,7 +161,7 @@ mutual
 theorem Ty.subst_ren {l m n} (σ : Subst l m) (ξ : Ren m n) :
     ∀ A : Ty l, (A.subst σ).ren ξ = A.subst (Tm.ren ξ ∘ σ)
   | .u .. => rfl
-  | .pi ⟨_, _⟩ _ => by simp only [Ty.subst, Ty.ren, Ty.subst_ren, Subst.ren_comp_up]
+  | .pi _ _ _ => by simp only [Ty.subst, Ty.ren, Ty.subst_ren, Subst.ren_comp_up]
   | .el .. => by simp only [Ty.subst, Ty.ren, Tm.subst_ren]
 
 theorem Tm.subst_ren {l m n} (σ : Subst l m) (ξ : Ren m n) :
@@ -169,9 +169,9 @@ theorem Tm.subst_ren {l m n} (σ : Subst l m) (ξ : Ren m n) :
   | .u' .. => rfl
   | .var _ => rfl
   | .const .. => rfl
-  | .lam ⟨_, _⟩ _ => by simp only [Tm.subst, Tm.ren, Ty.subst_ren, Tm.subst_ren, Subst.ren_comp_up]
+  | .lam _ _ _ => by simp only [Tm.subst, Tm.ren, Ty.subst_ren, Tm.subst_ren, Subst.ren_comp_up]
   | .app .. => by simp only [Tm.subst, Tm.ren, Tm.subst_ren]
-  | .pi' ⟨_, _⟩ _ => by simp only [Tm.subst, Tm.ren, Tm.subst_ren, Subst.ren_comp_up]
+  | .pi' _ _ _ => by simp only [Tm.subst, Tm.ren, Tm.subst_ren, Subst.ren_comp_up]
   | .proj .. => by simp only [Tm.subst, Tm.ren, Tm.subst_ren]
   | .letE .. => by simp only [Tm.subst, Tm.ren, Ty.subst_ren, Tm.subst_ren, Subst.ren_comp_up]
 
@@ -193,7 +193,7 @@ mutual
 theorem Ty.comp_subst {l m n} (σ : Subst l m) (τ : Subst m n) :
     ∀ A : Ty l, (A.subst σ).subst τ = A.subst (σ.comp τ)
   | .u .. => rfl
-  | .pi ⟨_, _⟩ _ => by simp only [Ty.subst, Ty.comp_subst, Subst.up_comp]
+  | .pi _ _ _ => by simp only [Ty.subst, Ty.comp_subst, Subst.up_comp]
   | .el .. => by simp only [Ty.subst, Tm.comp_subst]
 
 @[simp]
@@ -202,9 +202,9 @@ theorem Tm.comp_subst {l m n} (σ : Subst l m) (τ : Subst m n) :
   | .u' .. => rfl
   | .var .. => rfl
   | .const .. => rfl
-  | .lam ⟨_, _⟩ _ => by simp only [Tm.subst, Ty.comp_subst, Tm.comp_subst, Subst.up_comp]
+  | .lam _ _ _ => by simp only [Tm.subst, Ty.comp_subst, Tm.comp_subst, Subst.up_comp]
   | .app .. => by simp only [Tm.subst, Tm.comp_subst]
-  | .pi' ⟨_, _⟩ _ => by simp only [Tm.subst, Tm.comp_subst, Subst.up_comp]
+  | .pi' _ _ _ => by simp only [Tm.subst, Tm.comp_subst, Subst.up_comp]
   | .proj .. => by simp only [Tm.subst, Tm.comp_subst]
   | .letE .. => by simp only [Tm.subst, Ty.comp_subst, Tm.comp_subst, Subst.up_comp]
 
